src/goose_lang/recovery_adequacy.v
@@ -3,29 +3,59 @@ From iris.algebra Require Import auth.
 From iris.base_logic.lib Require Import proph_map.
 From iris.program_logic Require Export weakestpre adequacy.
 From Perennial.goose_lang Require Import proofmode notation.
-From Perennial.program_logic Require Import recovery_weakestpre.
+From Perennial.program_logic Require Import recovery_weakestpre recovery_adequacy.
 From Perennial.goose_lang Require Import typing adequacy.
 Set Default Proof Using "Type".
 
-Section recovery_adequacy.
+Section wpr_definitions.
 
 Context `{ffi_semantics: ext_semantics}.
 Context {ext_tys: ext_types ext}.
 Context `{!ffi_interp ffi}.
 
-Definition heap_namesO := leibnizO heap_names.
+Canonical Structure heap_namesO := leibnizO heap_names.
 Global Instance heapG_perennialG `{!heapG Σ} : perennialG heap_lang heap_crash_lang heap_namesO Σ :=
 {
   perennial_irisG := λ Hinv hnames, @heapG_irisG _ _ _ _ _ (heap_update _ _ Hinv (@pbundleT _ _ hnames));
   perennial_invG := λ _ _, eq_refl
 }.
 
-Section test.
-Context `{!heapG Σ}.
+End wpr_definitions.
 
-Remark test s k Hi Hc t E (e: expr heap_lang) rec Φ Φinv Φr :
-  wpr s k Hi Hc t E e rec Φ Φinv Φr -∗ True.
-Proof. eauto. Qed.
-
-End test.
-End recovery_adequacy.
+Theorem heap_recv_adequacy `{ffi_sem: ext_semantics} `{!ffi_interp ffi} {Hffi_adequacy:ffi_interp_adequacy} Σ `{!heapPreG Σ} `{crashPreG Σ} s k e r σ φ φr φinv Φinv :
+  (∀ `{Hheap : !heapG Σ} `{Hc: !crashG Σ} Hinv t,
+     (|={⊤}=>
+       (trace_frag σ.(trace) -∗ oracle_frag σ.(oracle) -∗
+       □ (∀ n σ κ, state_interp σ κ n ={⊤, ∅}=∗ ⌜ φinv σ ⌝) ∗
+       □ (∀ Hi t, Φinv Hi t -∗
+                       let _ := heap_update _ Hheap Hi (@pbundleT _ _ t) in
+                       □ ∀ σ κ n, state_interp σ κ n ={⊤, ∅}=∗ ⌜ φinv σ ⌝) ∗
+        wpr s k Hinv Hc t ⊤ e r (λ v, ⌜φ v⌝) Φinv (λ _ _ v, ⌜φr v⌝)))%I) →
+  recv_adequate (CS := heap_crash_lang) s e r σ (λ v _, φ v) (λ v _, φr v) φinv.
+Proof.
+  intros Hwp. eapply (wp_recv_adequacy_inv _ _ _ heap_namesO _ _).
+  iIntros (???) "".
+  iMod (gen_heap_init σ.(heap)) as (?) "Hh".
+  iMod (proph_map_init κs σ.(used_proph_id)) as (?) "Hp".
+  iMod (ffi_init _ _ σ.(world)) as (HffiG) "Hw".
+  iMod (trace_init σ.(trace) σ.(oracle)) as (HtraceG) "(Htr&Htrfrag&Hor&Hofrag)".
+  set (hG := (HeapG _ _ HffiG _ _ HtraceG)).
+  set (hnames := heap_get_names _ (HeapG _ _ HffiG _ _ HtraceG)).
+  iExists ({| pbundleT := hnames |}).
+  iExists
+    (λ t σ κs, let _ := heap_update_names Σ hG (@pbundleT _ _ t) in
+               state_interp σ κs O)%I,
+    (λ t _, True%I).
+  iExists (λ _ _, eq_refl).
+  iMod (Hwp hG Hc Hinv {| pbundleT := hnames |} with "[$] [$]") as "(#H1&#H2&Hwp)".
+  iModIntro.
+  iSplitR.
+  { iAlways. iIntros (??) "H". rewrite heap_get_update.
+    by iApply "H1".
+  }
+  iSplitR.
+  { iAlways. iIntros (??) "H". iDestruct ("H2" with "H") as "#H3".
+    iAlways. iIntros (??) "H". iMod ("H3" with "[$]"); eauto.
+  }
+  iFrame. rewrite //= ffi_get_update //=.
+Qed.
